 \subsection{Time--discretization of the linear case~(\ref{eq:quatre}) } Starting from  (\ref{eq:quatre}), let us introduce anew notation, \begin{equation}\begin{array}{l}M \dot{x}(t) = Ax(t) + r(t)  +b(t)\\[2mm]y(t) = h(x(t),\lambda (t),z) = Cx + Fz + D \lambda  \\[2mm]r(t) = g(t,\lambda (t) ) = B \lambda \\[2mm]\end{array}\label{sept-bis-bis}\end{equation}Let us now proceed with the time discretization of (\ref{sept-bis-bis}) by a fully implicit scheme : \begin{equation}  \begin{array}{l}    \label{eq:toto1}     M x^{\alpha+1}_{k+1} = M x_{k} +h\theta A x^{\alpha+1}_{k+1}+h(1-\theta) A x_k + h \theta _r r^{\alpha+1}_{k+1}+ h(1-\theta _r)r(t_k)  +b\\[2mm]     y^{\alpha+1}_{k+1} =  C x^{\alpha+1}_{k+1} + D \lambda ^{\alpha+1}_{k+1} +Fz +e\\[2mm]     r^{\alpha+1}_{k+1} = B \lambda ^{\alpha+1}_{k+1} \\[2mm]  \end{array}\end{equation}\[R_{free} = M(x^{\alpha}_{k+1} - x_{k}) -h\theta A x^{\alpha}_{k+1} - h(1-\theta) A x_k -hb_{k+1} \]\[R_{free} = W(x^{\alpha}_{k+1} - x_{k}) -h A x_{k} -hb_{k+1} \]\subsection{Resulting Newton step (only one step)}suppose:$\theta _r =1$\begin{equation}  \begin{array}{l}     (M -h\theta A)x^{\alpha+1}_{k+1} = M x_{k} +h(1-\theta) A x_k + r^{\alpha+1}_{k+1} + hb\\[2mm]     y^{\alpha+1}_{k+1} =  C x^{\alpha+1}_{k+1} + D \lambda ^{\alpha+1}_{k+1} +Fz + e \\[2mm]     r^{\alpha+1}_{k+1} = B \lambda ^{\alpha+1}_{k+1}\\[2mm]  \end{array}\end{equation}that lead to with: $ (M -h\theta A) = W$\begin{equation}  \begin{array}{l}     x^{\alpha+1}_{k+1} = W^{-1}(M x_{k} +h(1-\theta) A x_k + r^{\alpha+1}_{k+1} +hb) = xfree + W^{-1}(r^{\alpha+1}_{k+1})\\[2mm]     y^{\alpha+1}_{k+1} =  ( D+CW^{-1}B) \lambda ^{\alpha+1}_{k+1} +Fz + CW^{-1}(M x_k+h(1-\theta)Ax_k) +e \\[2mm]     r^{\alpha+1}_{k+1} = B \lambda ^{\alpha+1}_{k+1}\\[2mm]  \end{array}\end{equation}with $x_{free} = x^{\alpha}_{k+1} + W^{-1}(-R_{free})= x^{\alpha}_{k+1} - W^{-1}(W(x^{\alpha}_{k+1}- x_k) -hAx_k-hb_{k+1} )= W^{-1}(Mx_k +h(1-\theta)Ax_k +h b_{k+1})$\begin{equation}  \begin{array}{l}     y^{\alpha+1}_{k+1} =  ( D+CW^{-1}B) \lambda ^{\alpha+1}_{k+1} +Fz + Cx_{free}+e\\[2mm]     r^{\alpha+1}_{k+1} = B \lambda ^{\alpha+1}_{k+1}\\[2mm]  \end{array}\end{equation}\subsection{coherence with previous formulation}\[y_p = y^{\alpha}_{k+1} -\mathcal R^{\alpha}_{yk+1} + C^{\alpha}_{k+1}(x_p -x^{\alpha}_{k+1}) -D^{\alpha}_{k+1} \lambda^{\alpha}_{k+1} \]\[y_p = Cx_k + D \lambda _k  + C(\tilde x_{free}) -D \lambda_k +Fz + e\]\[y_p = Cx_k   + C(\tilde x_{free})  +Fz + e\]\[y_p = Cx_k   + C(\tilde x_{free})  +Fz + e\]\[y_p = C(x_{free})  +Fz + e\]%In the case of the system~(\ref{eq:deux}) with a affine function $f$ or $\theta =0$, the the MLCP matrix $W$ can be computed before the beginning of the time loop saving a lot of computing effort.  In the case of the system (\ref{eq:trois}) with $\theta=\gamma=0$, the MLCP matrix $W$ can be computed before the beginning of the Newton loop.\clearpage%%% Local Variables: %%% mode: latex%%% TeX-master: "EulerSliding"%%% End: 