\subsection{Time--discretization of the the case~(\ref{eq:quatre}) } This case is implemented in Siconos with the relation FirstOrderType2R.Starting from  (\ref{eq:quatre}), let us introduce a new notation, \begin{equation}\begin{array}{l}M \dot{x}(t) = f(x(t),t) + r(t)  \\[2mm]y(t) = h(t,x(t),\lambda (t)) \\[2mm]r(t) = g(t,\lambda (t) ) \\[2mm]\end{array}\label{sept-bis-bis}\end{equation}Let us now proceed with the time discretization of (\ref{sept-bis-bis}) by a fully implicit scheme : \begin{equation}  \begin{array}{l}    \label{eq:toto1}     M x_{k+1} = M x_{k} +h\theta f(x_{k+1},t_{k+1})+h(1-\theta) f(x_k,t_k) + h \theta _r r(t_{k+1})     + h(1-\theta _r)r(t_k)  \\[2mm]     y_{k+1} =  h(t+1,x_{k+1},\lambda _{k+1}) \\[2mm]     r_{k+1} = g(\lambda_{k+1},t+1)\\[2mm]  \end{array}\end{equation}\subsection{Newton's linearization} \paragraph{Newton's linearization} The first line of the  problem~(\ref{eq:toto1}) can be written under the form of a residue $\mathcal R$ depending only on $x_{k+1}$ and $r_{k+1}$ such that \begin{equation}  \label{eq:NL23}  \mathcal R (x_{k+1},r _{k+1}) =0\end{equation}with $\mathcal R(x,r) = M (x - x_{k}) -h\theta f( x , t_{k+1}) - h(1-\theta)f(x_k,t_k) - h\theta _r r- h(1-\theta_r)r_k$.The solution of this system of nonlinear equations is sought as a limit of the sequence $\{ x^{\alpha}_{k+1},r^{\alpha}_{k+1} \}_{\alpha \in \NN}$ such that \begin{equation}   \label{eq:NL27}   \begin{cases}     x^{0}_{k+1} = x_k \\ \\     \mathcal R_L( x^{\alpha+1}_{k+1},r^{\alpha+1}_{k+1}) = \mathcal     R(x^{\alpha}_{k+1},r^{\alpha}_{k+1})  + \left[ \nabla_{x} \mathcal     R(x^{\alpha}_{k+1},r^{\alpha}_{k+1})\right] (x^{\alpha+1}_{k+1}-x^{\alpha}_{k+1} ) +     \left[ \nabla_{x} \mathcal R(x^{\alpha}_{k+1},r^{\alpha}_{k+1})\right] (r^{\alpha+1}_{k+1} - r^{\alpha}_{k+1} ) =0 \end{cases}\end{equation}The residu free is also defined (useful for implementation only):\[\mathcal R _{free}(x) =  M (x - x_{k}) -h\theta f( x , t_{k+1}) - h(1-\theta)f(x_k,t_k)\]\[\mathcal R (x,r) = \mathcal R _{free}(x)   - h\theta _r r - h(1-\theta_r)r_k\]\[ \fbox{$\mathcal R^{\alpha}_{k+1} = \mathcal R (x^{\alpha}_{k+1},r^{\alpha}_{k+1}) = \mathcal R_{free}(x^{\alpha}_{k+1},r^{\alpha}_{k+1} )  - h\theta _r r^{\alpha}_{k+1} - h(1-\theta_r)r_k$}\]\[ \mathcal R _{free k+1} ^{\alpha} = \mathcal R_{free}(x^{\alpha}_{k+1},r^{\alpha}_{k+1} )=\fbox{$M(x^{\alpha}_{k+1} - x_{k}) -h\theta f( x^{\alpha}_{k+1} , t_{k+1}) - h(1-\theta)f(x_k,t_k)$}\] The computation of the Jacobian of $\mathcal R$ with respect to $x$, denoted by $M(x,\lambda)$ leads to \begin{equation}   \label{eq:NL29}   \begin{array}{l}    W^{\alpha}_{k+1}= \nabla_{x} \mathcal R (x^{\alpha}_{k+1},r^{\alpha}_{k+1})= M - h  \theta \nabla_{x} f(  x^{\alpha}_{k+1}, t_{k+1} ).\\ \end{array}\end{equation}At each time--step, we have to solve the following linearized problem,\begin{equation}   \label{eq:NL210}    \mathcal R^{\alpha}_{k+1} + W^{\alpha}_{k+1} (x^{\alpha+1}_{k+1} -    x^{\alpha}_{k+1}) - h \theta _r (r^{\alpha+1}_{k+1} - r^{\alpha}_{k+1} )  =0 ,\end{equation}that is\begin{equation}   \begin{array}{l} h \theta _r  r^{\alpha+1}_{k+1} = r_c + W^{\alpha}_{k+1} x^{\alpha+1}_{k+1} .\label{eq:NL211}  \end{array}\end{equation}with \begin{equation}   \begin{array}{l}r_c = h \theta _r r^{\alpha}_{k+1} - W^{\alpha}_{k+1} x^{\alpha}_{k+1} + \mathcal R^{\alpha}_{k+1}=- W^{\alpha}_{k+1} x^{\alpha}_{k+1} + \mathcal R_{free k+1} ^{\alpha} - h(1-\theta_r)r_k \end{array}   \end{equation}so:\[x^{\alpha+1}_{k+1} = h(W^{\alpha}_{k+1})^{-1}r^{\alpha+1}_{k+1} +(W^{\alpha}_{k+1})^{-1}(\mathcal R_{free k+1} ^{\alpha})+x^{\alpha}_{k+1}\]\[\fbox{$x^{\alpha+1}_{k+1} = h(W^{\alpha}_{k+1})^{-1}r^{\alpha+1}_{k+1} +x_{free}$}\]The matrix $W$ is clearly non singular for small $h$.The same operation is performed with the second equation of (\ref{eq:toto1})\begin{equation}   \label{eq:NL29}   \begin{array}{l}      \mathcal R_y(x,y,\lambda)=y-h(t_{k+1},x,\lambda) =0\\ \\      \mathcal R_{Ly}(x^{\alpha+1}_{k+1},y^{\alpha+1}_{k+1},\lambda^{\alpha+1}_{k+1}) = \mathcal      R_{y}(x^{\alpha}_{k+1},y^{\alpha}_{k+1},\lambda^{\alpha}_{k+1}) +      (y^{\alpha+1}_{k+1}-y^{\alpha}_{k+1})- \\ \qquad \qquad      C^{\alpha}_{k+1}(x^{\alpha+1}_{k+1}-x^{\alpha}_{k+1}) - D^{\alpha}_{k+1}(\lambda^{\alpha+1}_{k+1}-\lambda^{\alpha}_{k+1})=0\\       \end{array}\end{equation}$\mathcal R_y(x^{\alpha+1}_{k+1},y^{\alpha+1}_{k+1},\lambda^{\alpha+1}_{k+1})$ leading to the following linearized equation\begin{equation}  y^{\alpha+1}_{k+1} =  y^{\alpha}_{k+1}  -\mathcal R^{\alpha}_{yk+1}+ \\  C^{\alpha}_{k+1}(x^{\alpha+1}_{k+1}-x^{\alpha}_{k+1}) +  D^{\alpha}_{k+1}(\lambda^{\alpha+1}_{k+1}-\lambda^{\alpha}_{k+1}). \label{eq:NL211y}\end{equation}with,\begin{equation}     \begin{array}{l}  C^{\alpha}_{k+1} = \nabla_xh(t_{k+1}, x^{\alpha}_{k+1},\lambda^{\alpha}_{k+1} ) \\ \\  D^{\alpha}_{k+1} = \nabla_{\lambda}h(t_{k+1}, x^{\alpha}_{k+1},\lambda^{\alpha}_{k+1}) \end{array}\end{equation}and\begin{equation}\fbox{$\mathcal R^{\alpha}_{yk+1} = y^{\alpha}_{k+1} - h(x^{\alpha}_{k+1},\lambda^{\alpha}_{k+1},t_{k+1})$} \end{equation}The same operation is performed with the thirdtheta equation of (\ref{eq:toto1})\begin{equation}   \label{eq:NL29}   \begin{array}{l}      \mathcal R_r(r,\lambda)=r-g(\lambda,t_{k+1}) =0\\ \\      \mathcal R_{L\lambda}(r^{\alpha+1}_{k+1},\lambda^{\alpha+1}_{k+1}) = \mathcal      R_{rk+1}^{\alpha} + (r^{\alpha+1}_{k+1} - r^{\alpha}_{k+1}) -      B^{\alpha}_{k+1}(\lambda^{\alpha+1}_{k+1} -      \lambda^{\alpha}_{k+1})=0\\ \\      r^{\alpha+1}_{k+1} = - \mathcal R_{rk+1}^{\alpha} + r^{\alpha}_{k+1} + B^{\alpha}_{k+1}(\lambda^{\alpha+1}_{k+1} -      \lambda^{\alpha}_{k+1})\\ \\      \fbox{$r^{\alpha+1}_{k+1} = g(\lambda ^{\alpha}_{k+1},t_{k+1}) -B^{\alpha}_{k+1}      \lambda^{\alpha}_{k+1} + B^{\alpha}_{k+1} \lambda^{\alpha+1}_{k+1}$}        \end{array}\end{equation}because the r residue is:\begin{equation}\mathcal      R_{rk+1}^{\alpha} = r^{\alpha}_{k+1} - g(r^{\alpha}_{k+1},t_{k+1})  \end{equation}with,\begin{equation}     \begin{array}{l}  B^{\alpha}_{k+1} = \nabla_{\lambda}g(r^{\alpha}_{k+1},t_{k+1}) \end{array}\end{equation}Inserting (\ref{eq:NL211}), we get the following linear relation between $x^{\alpha+1}_{k+1}$ and$\lambda^{\alpha+1}_{k+1}$, \begin{equation}   \begin{array}{l}    (W^{\alpha}_{k+1})x^{\alpha+1}_{k+1} = h \theta _r \left[ g(r^{\alpha}_{k+1},t_{k+1}) +    B^{\alpha}_{k+1} (\lambda^{\alpha+1}_{k+1} - \lambda^{\alpha}_{k+1}) \right] -r_c \\ \\    x^{\alpha+1}_{k+1} = h \theta _r (W^{\alpha}_{k+1})^{-1}\left[ g(r^{\alpha}_{k+1},t_{k+1}) + B^{\alpha}_{k+1} (\lambda^{\alpha+1}_{k+1} - \lambda^{\alpha}_{k+1}) \right] -(W^{\alpha}_{k+1})^{-1}(- W^{\alpha}_{k+1} x^{\alpha}_{k+1} + \mathcal R_{free k+1} ^{\alpha} - h(1-\theta_r)r_k) \\ \\    x^{\alpha+1}_{k+1} =  x_p + h \theta _r (W^{\alpha}_{k+1})^{-1}  B^{\alpha}_{k+1}    \lambda^{\alpha+1}_{k+1}    \end{array}\end{equation}with $\theta _r =1$:\[(W^{\alpha}_{k+1})x^{\alpha+1}_{k+1}= hr^{\alpha+1}_{k+1}- \mathcal R_{free k+1} ^{\alpha}+W^{\alpha}_{k+1})x^{\alpha}_{k+1}\]\[x^{\alpha+1}_{k+1}= h(W^{\alpha}_{k+1})^{-1}r^{\alpha+1}_{k+1}- (W^{\alpha}_{k+1})^{-1} \mathcal R_{free k+1} ^{\alpha}+x^{\alpha}_{k+1}\]\[x^{\alpha+1}_{k+1}= h(W^{\alpha}_{k+1})^{-1}r^{\alpha+1}_{k+1}+x_{free}\]with\begin{equation}x_p - x^{\alpha}_{k+1} =  (W^{\alpha}_{k+1})^{-1}  \left[ -r_c + h \theta _r( g(r^{\alpha}_{k+1},t_{k+1}) -      B^{\alpha}_{k+1} \lambda^{\alpha}_{k+1} \right)]  \end{equation}\[ x_p - x^{\alpha}_{k+1} = \tilde x_{free} + h \theta _r(W^{\alpha}_{k+1})^{-1}( g(r^{\alpha}_{k+1},t_{k+1}) -      B^{\alpha}_{k+1} \lambda^{\alpha}_{k+1} ) \]      \[    \tilde x_{free}= (W^{\alpha}_{k+1})^{-1}(-      \mathcal R _{free k+1} ^{\alpha} +h(1-\theta _r)r_k)\]      \[x_{free} = \tilde x_{free} + x^{\alpha}_{k+1}=\fbox{$-W^{-1}R_{free k+1} ^{\alpha} + x^{\alpha}_{k+1}$}\]\[ \fbox{$x_p  = x_{free} + h \theta _r(W^{\alpha}_{k+1})^{-1}( g(\lambda ^{\alpha}_{k+1},t_{k+1}) -      B^{\alpha}_{k+1} \lambda^{\alpha}_{k+1} )$} \]    Inserting (\ref{eq:NL211y}), we get the following linear relation between $y^{\alpha+1}_{k+1}$ and $\lambda^{\alpha+1}_{k+1}$, \begin{equation}   \begin{array}{l} y^{\alpha+1}_{k+1} = y_p + \left[ h \theta _r C^{\alpha}_{k+1} (W^{\alpha}_{k+1})^{-1}  B^{\alpha}_{k+1} + D^{\alpha}_{k+1} \right]\lambda^{\alpha+1}_{k+1}   \end{array}\end{equation}with \begin{equation}\fbox{$y_p = y^{\alpha}_{k+1} -\mathcal R^{\alpha}_{yk+1} + C^{\alpha}_{k+1}(x_p -x^{\alpha}_{k+1}) -D^{\alpha}_{k+1} \lambda^{\alpha}_{k+1} $}\end{equation}\begin{equation}y_p = h(x^{\alpha}_{k+1},\lambda^{\alpha}_{k+1}) + C^{\alpha}_{k+1}(x_p -x^{\alpha}_{k+1}) -D^{\alpha}_{k+1} \lambda^{\alpha}_{k+1} \end{equation}\begin{equation}y_p = h(x^{\alpha}_{k+1},\lambda^{\alpha}_{k+1}) - C^{\alpha}_{k+1}x^{\alpha}_{k+1}+C^{\alpha}_{k+1} x_{free} +hC(W^{\alpha}_{k+1})^{-1}(g(\lambda^{\alpha}_{k+1},t_{k+1})-B^{\alpha}_{k+1} \lambda^{\alpha}_{k+1}) -D^{\alpha}_{k+1} \lambda^{\alpha}_{k+1} \end{equation}\paragraph{Mixed linear complementarity problem (MLCP)}To summarize, the problem to be solved in each Newton iteration is:\\{  \begin{minipage}[l]{1.0\linewidth}    \begin{equation}      \begin{cases}      \begin{array}[l]{l}        y^{\alpha+1}_{k+1} =   \tilde W^{\alpha}_{k+1}  \lambda^{\alpha+1}_{k+1} + b^{\alpha}_{k+1}        \\ \\        -y^{\alpha+1}_{k+1} \in N_{[l,u]}(\lambda^{\alpha+1}_{k+1} ).       \end{array}      \label{eq:NL214}      \end{cases}    \end{equation}  \end{minipage}}with $W\in \RR^{m\times m}$ and $b\in\RR^{m}$ defined by\begin{equation}  \label{eq:NL215} \begin{array}[l]{l}   \tilde W^{\alpha}_{k+1} = h \theta _r C^{\alpha}_{k+1} (W^{\alpha}_{k+1})^{-1}  B^{\alpha}_{k+1} + D^{\alpha}_{k+1} \\   b^{\alpha}_{k+1} = y_p\end{array}\end{equation}The problem~(\ref{eq:NL214}) is equivalent to a Mixed Linear Complementarity Problem (MLCP) which can be solved under suitable assumptions by many linear complementarity solvers such as pivoting techniques, interior point techniques and splitting/projection strategies. The  reformulation into a standard MLCP follows the same line as for the MCP in the previous section. One obtains,    \begin{equation}      \begin{array}[l]{l}        y^{\alpha+1}_{k+1} =   - W^{\alpha}_{k+1}  \lambda^{\alpha+1}_{k+1} + b^{\alpha}_{k+1}        \\ \\        (y^{\alpha+1}_{k+1})_i  = 0 \qquad \textrm{ for } i \in \{ 1..n\}\\[2mm]        0 \leq  (\lambda^{\alpha+1}_{k+1})_i\perp (y^{\alpha+1}_{k+1})_i \geq 0 \qquad \textrm{ for } i \in \{ n..n+m\}\\      \end{array}      \label{eq:MLCP1}     \end{equation}\paragraph{MLCP solvers.} As for MCP, there exists numerous methods to numerically solve MLCP. In the worst case when the matrix $W^{\alpha+1}_{k+1}$ has no special properties, the MCLP can be always solved by enumerative solvers for which various implementation can be found. With positivity, P-matrix  or co-positivity properties, standard methods for LCP\cite{Cottle.Pang.ea1992} can be straightforwardly extended. Among these methods, we can cite the family of projection/splitting methods, interior point methods and semi-smooth Newton methods (see \cite{acary2008} for an overview of various types of methods.).\subsection{Implementation In siconos}The initial residu x:\[\mathcal   R^{0}_{k+1}= \mathcal   R^{0}_{free k+1}-hr^{0}_{k+1}\]\[\mathcal   R^{0}_{k+1}= M(x^{0}_{k+1} - x_k) -h\theta f(x_k,t_{k+1})-h(1-\theta)f(x_k,t_k)-hr^{0}_{k+1}\]\[\mathcal   R^{0}_{k+1}= -h\theta f(x_k,t_{k+1})-h(1-\theta)f(x_k,t_k)-hr^{0}_{k+1}\]The initial residu y:\[\mathcal   R^{0}_{y k+1} =y_k -h(x_k,\lambda _k,t_{k+1})\]The initial residu r:\[\mathcal   R^{0}_{r k+1} =r_k -g(\lambda _k,t_{k+1})\]%\subsection{Algorithms} %We propose in this section two algorithms to sum-up the numerical implementation of the implicit%Euler time--stepping scheme.%The Algorithm~\ref{Algo:EulerSliding-MCP} describes the implementation%with a generic MCP solvers and%The Algorithm~\ref{Algo:EulerSliding-MCLP} describes the  numerical implementation of the algorithm with an external Newton linearization and a MCLP solver.%\begin{algorithm}[htbp]%   \begin{algorithmic}% { \sf %    \REQUIRE $x_k, x^{\alpha+1}_{k+1},\lambda ^{\alpha+1}_{k+1} ,\lambda ^{\alpha}_{k+1},g^{\alpha}_{k+1} $ %    \ENSURE  $g^{\alpha+1}_{k+1}, r^{\alpha+1}_{k+1}, R^{\alpha+1}_{k+1},  Rfree^{\alpha+1}_{k+1}, Rr^{\alpha+1}_{k+1}$%    \STATE $r^{\alpha+1}_{k+1} = g^{\alpha}_{k+1} +B^{\alpha}_{k+1} (\lambda^{\alpha+1}_{k+1} -\lambda ^{\alpha}_{k+1})$%    \STATE $ Rfree^{\alpha+1}_{k+1} = M(x^{\alpha+1}_{k+1}-x_k)-h \theta f(x^{\alpha+1}_{k+1},t_{k+1})-h(1-\theta)f(x_k,t_k)$%    \STATE $ R^{\alpha+1}_{k+1} = M(x^{\alpha+1}_{k+1}-x_k)-h \theta%    f(x^{\alpha+1}_{k+1},t_{k+1})-h(1-\theta)f(x_k,t_k) -hr^{\alpha+1}_{k+1}$%     \STATE $g^{\alpha+1}_{k+1} = g(\lambda ^{\alpha+1}_{k+1},t_{k+1})$%     \STATE $Rr^{\alpha+1}_{k+1} =r^{\alpha+1}_{k+1} - g^{\alpha+1}_{k+1} $%     %     \STATE $ \sf$}%   \end{algorithmic}%   \caption{compute Residu x and r}  % \label{Algo:ResiduXandR}%\end{algorithm}%\begin{algorithm}[htbp]%   \begin{algorithmic}% { \sf %    \REQUIRE $x^{\alpha+1}_{k+1}, \lambda^{\alpha+1}_{k+1}$ %    \ENSURE  $h^{\alpha+1}_{k+1},Ry^{\alpha+1}_{k+1}$%     \STATE $ h^{\alpha+1}_{k+1}=h(x^{\alpha+1}_{k+1},\lambda^{\alpha+1}_{k+1},t_{k+1})$%     \STATE $ Ry^{\alpha+1}_{k+1}=y^{\alpha+1}_{k+1} -h^{\alpha+1}_{k+1} $%     \STATE $ \sf$}%   \end{algorithmic}%   \caption{compute Residu y }  % \label{Algo:Residuy}%\end{algorithm}%%%\begin{algorithm}[htbp]%   \begin{algorithmic}% { \sf %    \REQUIRE System definition: $\sf f, g, h$ %    \REQUIRE $\sf x(0)$ the initial condition%    \REQUIRE $\sf t_0, T$ time--integration interval%    \REQUIRE $\sf h$ time--step%    \REQUIRE $\sf \theta, \gamma$ numerical integration parameters %    \REQUIRE $\sf \varepsilon $ Newton's method tolerance%    \ENSURE  $\sf (\{ x_k\}, \{ \lambda_k\},\{y_k \}), k \in\{1,2, \ldots \}$ %    \STATE $ \sf $%    \STATE $\sf k \leftarrow 0;\quad  x^0_0 \leftarrow x(0);\quad \sf y^0_0 \leftarrow 0;\quad \sf%    \lambda^0_0 \leftarrow 0; \sf g^0_0 \leftarrow g(0,0) $  %    \STATE $ $%    \STATE //\textit{ Time integration loop}%     \WHILE {$\sf t_k < T$}%         \STATE $x_k = x^{\alpha}_k$%         \STATE $\sf \alpha \leftarrow 0;\quad\sf x^0_{k+1} ; \sf \lambda%    ^0_{k+1}; \sf y^0_{k+1}; \sf g^{\alpha}_{k+1}$%        \STATE  computeResiduXandR \\%        \STATE  computeResiduY \\%        \STATE //\textit{Newton's loop}%          \WHILE {$\sf  \| R^{0}_{k+1}\|+\| Ry^{0}_{k+1}\|+\| Rr^{0}_{k+1}\| > \varepsilon$}  %         \STATE  $x_{free}=x^{\alpha}_{k+1} -(W^{\alpha}_{k+1})^{-1}(\mathcal R^{alpha}_{free k+1})$%         \STATE  $x_p=x_{free}+h(W^{\alpha}_{k+1})^{-1}(g^{\alpha}_{k+1} -B^{\alpha}_{k+1} \lambda ^{\alpha}_{k+1})$%         \STATE $y_p=h^{\alpha}_{k+1} -%          C^{\alpha}_{k+1}x^{\alpha}_{k+1}+C^{\alpha}_{k+1}x_{free}+hC^{\alpha}_{k+1}(W^{\alpha}_{k+1})^{-1}(g^{\alpha}_{k+1}-B\lambda%          ^{\alpha}_{k+1})-D^{\alpha}_{k+1} \lambda ^{\alpha}_{k+1}$%         \STATE Solve the MLCP, ie get $y^{\alpha+1}_{k+1}$ and $\lambda ^{\alpha}_{k+1}$.%         \STATE $x^{\alpha+1}_{k+1} = x_p+h(W^{\alpha}_{k+1})^{-1}B^{\alpha}_{k+1} \lambda%         ^{\alpha}_{k+1}$%         \STATE call computeResiduXandR \\%         \STATE call computeResiduY \\%         \STATE $\alpha = \alpha +1$\\%         \ENDWHILE%      \STATE $x_k = x^{\alpha}_k$%      \ENDWHILE%     \STATE $ \sf$}%   \end{algorithmic}%   \caption{Implicit Euler time-discretization with an external Newton loop and a MLCP solver }  % \label{Algo:EulerSliding-MCLP}%\end{algorithm}In the case of the system~(\ref{eq:deux}) with a affine function $f$ or $\theta =0$, the the MLCP matrix $W$ can be computed before the beginning of the time loop saving a lot of computing effort.  In the case of the system (\ref{eq:trois}) with $\theta=\gamma=0$, the MLCP matrix $W$ can be computed before the beginning of the Newton loop.\clearpage%%% Local Variables: %%% mode: latex%%% TeX-master: "EulerSliding"%%% End: 